Make some progress reasoning about blocks
The disk model is definitely messy and should be fixed to more closely
resemble in-memory values. The only caveat is that we shouldn't change
the underlying state type for disks too drastically (currently it's
reasonable, a map from Z to (vec u8 4096)). Ideally all the changes
would happen in the state interpretation, we do one proof of soundness
against the semantics, and after that we have nicer points-to facts.

I'm thinking that we should start thinking of the disks as being
byte-based, with the 4096-byte blocks being an invariant of the size
(already the lack of holes is an invariant) and with reads and writes
being atomic over 4096 addresses simultaneously.

src/go_lang/examples/proof/append_log_proof.v
@@ -8,7 +8,7 @@ Import uPred.
 
 Section heap.
 Context `{!heapG Σ}.
-Context `{!diskG Σ}.
+Existing Instance diskG0.
 Implicit Types P Q : iProp Σ.
 Implicit Types Φ : val → iProp Σ.
 Implicit Types Δ : envs (uPredI (iResUR Σ)).
@@ -16,6 +16,54 @@ Implicit Types v : val.
 Implicit Types z : Z.
 Implicit Types s : Slice.t.
 Implicit Types stk : stuckness.
+
+Lemma slice_to_block_array s b :
+  is_slice s (Block_to_vals b) ⊣⊢ mapsto_block s.(Slice.ptr) 1 b.
+Proof.
+  rewrite /mapsto_block /is_slice /array.
+  (* TODO: how to relate two different big_ops? *)
+Admitted.
+
+Transparent disk.Read disk.Write.
+
+Theorem wp_Write stk E (a: u64) s b :
+  {{{ ▷ ∃ b0, int.val a d↦ b0 ∗ is_slice s (Block_to_vals b) }}}
+    Write #a (slice_val s) @ stk; E
+  {{{ RET #(); int.val a d↦ b ∗ is_slice s (Block_to_vals b) }}}.
+Proof.
+  iIntros (Φ) ">Hpre HΦ".
+  iDestruct "Hpre" as (b0) "[Hda Hs]".
+  wp_call.
+  wp_call.
+  wp_apply (wp_WriteOp with "[Hda Hs]").
+  { iIntros "!>".
+    iExists b0.
+    iFrame.
+    by iApply slice_to_block_array. }
+  iIntros "[Hda Hmapsto]".
+  iApply "HΦ".
+  iFrame.
+  by iApply slice_to_block_array.
+Qed.
+
+Definition val_to_byte (v: val): u8 :=
+  match v with
+  | LitV (LitByte x) => x
+  | _ => 0
+  end.
+
+Definition list_to_block (l: list val) (H: length l = Z.to_nat 4096) : Block :=
+  eq_rect _ _ (vmap val_to_byte (Vector.of_list l)) _ H.
+
+Lemma array_to_block l vs :
+  (* TODO: only true if vs are all actually bytes (otherwise roundtripping
+  produces #(U8 0) and not the original value) *)
+  l ↦∗ vs ∗ ⌜length vs = Z.to_nat 4096⌝ -∗ ∃ H, mapsto_block l 1 (list_to_block vs H).
+Proof.
+  rewrite /array /mapsto_block /Block_to_vals /list_to_block.
+  iIntros "[Hl %]".
+  iExists H.
+Admitted.
 
 Definition is_hdr (sz disk_sz: u64): iProp Σ :=
   ∃ b, 0 d↦ b ∗
@@ -30,5 +78,99 @@ Definition is_log (v:val) (vs:list Block): iProp Σ :=
     (∃ (free: list Block), (1 + length vs) d↦∗ free ∗
     ⌜ (1 + length vs + length free)%Z = int.val disk_sz ⌝)
 .
+
+Ltac mia :=
+  change (int.val 1) with 1;
+  change (int.val 4) with 4;
+  change (int.val 8) with 8;
+  change (int.val 4096) with 4096;
+  lia.
+
+Theorem wp_write_hdr stk E (sz0 disk_sz0 sz disk_sz:u64) :
+  {{{ is_hdr sz0 disk_sz0 }}}
+    Log__writeHdr (#sz, #disk_sz)%V @ stk; E
+  {{{ RET #(); is_hdr sz disk_sz }}}.
+Proof.
+  iIntros (Φ) "Hhdr HΦ".
+  iDestruct "Hhdr" as (b) "(Hd0&%&%)".
+  wp_call.
+  wp_call.
+  wp_alloc l as "Hs"; first mia.
+  wp_steps.
+  wp_call.
+  wp_call.
+  wp_bind (UInt64Put _ _).
+  rewrite slice_val_fold.
+  wp_apply (wp_UInt64Put with "[Hs]").
+  { iFrame.
+    rewrite replicate_length /=.
+    iPureIntro; mia. }
+  iIntros "Hs".
+  wp_steps.
+  wp_call.
+  wp_bind (SliceSkip _ _).
+  wp_apply (wp_SliceSkip with "[$Hs]").
+  { iPureIntro.
+    rewrite app_length drop_length replicate_length u64_le_bytes_length.
+    mia. }
+  cbv [Slice.ptr Slice.sz slice_skip].
+  iIntros "[Hrest Htake]".
+  rewrite take_app_le ?drop_app_ge.
+  { wp_bind (UInt64Put _ _).
+    wp_apply (wp_UInt64Put with "[Hrest]").
+    { iSplitL.
+      { rewrite drop_drop drop_replicate.
+        rewrite u64_le_bytes_length.
+        match goal with
+        | |- context[replicate ?n _] => change n with (Z.to_nat 4088)
+        end.
+        change (word.sub 4096 8) with (U64 4088).
+        iExact "Hrest". }
+      iPureIntro.
+      rewrite replicate_length; mia.
+    }
+    rewrite drop_replicate.
+    change (Z.to_nat 4088 - 8)%nat with (Z.to_nat 4080).
+    iIntros "Hrest".
+    wp_steps.
+    iDestruct "Hrest" as "[Hskip _]".
+    cbv [Slice.ptr].
+    rewrite firstn_all2; rewrite ?u64_le_bytes_length; last mia.
+    iDestruct (array_app with "[$Htake $Hskip]") as "Hl".
+    iDestruct (array_to_block with "[$Hl]") as (Hlength) "Hb".
+    { iPureIntro.
+      rewrite ?app_length ?u64_le_bytes_length replicate_length.
+      reflexivity. }
+    wp_apply (wp_Write with "[Hd0 Hb]").
+    { iExists b.
+      iModIntro.
+      iSplitL "Hd0"; [ iFrame | ].
+      iDestruct (slice_to_block_array (Slice.mk l 4096) with "[$Hb]") as "Hs".
+      iExact "Hs". }
+    iIntros "[Hd0 Hs]".
+    iApply "HΦ".
+    rewrite /is_hdr.
+    iExists _; iFrame "Hd0".
+    iPureIntro.
+    admit. }
+  { rewrite u64_le_bytes_length; mia. }
+  { rewrite u64_le_bytes_length; mia. }
+Admitted.
+
+Theorem wp_init stk E (sz: u64) vs :
+  {{{ 0 d↦∗ vs ∗ ⌜length vs = int.nat sz⌝ }}}
+    Init #sz @ stk; E
+  {{{ v (ok: bool), RET (v, #ok); ⌜ok⌝ -∗ is_log v [] }}}.
+Proof.
+  iIntros (Φ) "[Hdisk %] HΦ".
+  wp_lam.
+  wp_pures.
+  wp_if_destruct; wp_pures.
+  - iApply "HΦ".
+    iIntros ([]).
+  - rewrite word.unsigned_ltu in Heqb.
+    apply Z.ltb_ge in Heqb.
+    wp_lam.
+Abort.
 
 End heap.
