src/go_lang/slice.v
@@ -98,10 +98,10 @@ Proof.
   typecheck.
 Qed.
 
+(* TODO: it would be nice if we could panic in the model if this goes
+out-of-bounds, but it seems we need to unfold the definition to use it *)
 Definition SliceSkip: val :=
-  λ: "s" "n", if: "n" ≤ slice.len "s"
-              then (slice.ptr "s" +ₗ "n", slice.len "s" - "n")
-              else Panic "skip: slice index out-of-bounds".
+  λ: "s" "n", (slice.ptr "s" +ₗ "n", slice.len "s" - "n").
 
 Theorem SliceSkip_t t : ⊢ SliceSkip : (slice.T t -> uint64T -> slice.T t).
 Proof.
